Spit boilerplate for every subcase of the fundamental lemma.

theories/Fundamental.v
@@ -8,27 +8,23 @@ Set Universe Polymorphism.
 
 (* FundCon, FundTy, ... are parameterized by a tag with a bunch of typing 
   judgment predicates *)
-Definition FundCon `{ta : tag} `{WfContext ta} `{WfType ta} `{Typing ta}
-  `{ConvType ta} `{ConvTerm ta} `{ConvNeu ta} `{RedType ta} `{RedTerm ta}
+Definition FundCon `{GenericTypingProperties}
   (Γ : context) : Type := [||-v Γ ].
 
 Module FundTy.
-  Record FundTy `{ta : tag} `{WfContext ta} `{WfType ta} `{Typing ta}
-    `{ConvType ta} `{ConvTerm ta} `{ConvNeu ta} `{RedType ta} `{RedTerm ta}
-    {Γ : context} {A : term} 
+  Record FundTy `{GenericTypingProperties} {Γ : context} {A : term} 
   : Type := {
     VΓ : [||-v Γ ];
     VA : [ Γ ||-v< one > A | VΓ ]
   }.
   
-  Arguments FundTy {_ _ _ _ _ _ _ _ _}.
-End FundTy. 
+  Arguments FundTy {_ _ _ _ _ _ _ _ _ _ _ _}.
+End FundTy.
 
 Export FundTy(FundTy,Build_FundTy).
 
 Module FundTyEq.
-  Record FundTyEq `{ta : tag} `{WfContext ta} `{WfType ta} `{Typing ta}
-    `{ConvType ta} `{ConvTerm ta} `{ConvNeu ta} `{RedType ta} `{RedTerm ta}
+  Record FundTyEq `{GenericTypingProperties}
     {Γ : context} {A B : term}
   : Type := {
     VΓ : [||-v Γ ];
@@ -36,28 +32,26 @@ Module FundTyEq.
     VB : [ Γ ||-v< one > B | VΓ ];
     VAB : [ Γ ||-v< one > A ≅ B | VΓ | VA ]
   }.
-  Arguments FundTyEq {_ _ _ _ _ _ _ _ _}.  
+  Arguments FundTyEq {_ _ _ _ _ _ _ _ _ _ _ _}.
 End FundTyEq.
 
 Export FundTyEq(FundTyEq,Build_FundTyEq).
 
 Module FundTm.
-  Record FundTm `{ta : tag} `{WfContext ta} `{WfType ta} `{Typing ta}
-    `{ConvType ta} `{ConvTerm ta} `{ConvNeu ta} `{RedType ta} `{RedTerm ta}
+  Record FundTm `{GenericTypingProperties}
     {Γ : context} {A t : term}
   : Type := {
     VΓ : [||-v Γ ];
     VA : [ Γ ||-v< one > A | VΓ ];
     Vt : [ Γ ||-v< one > t : A | VΓ | VA ];
   }.
-  Arguments FundTm {_ _ _ _ _ _ _ _ _}.  
+  Arguments FundTm {_ _ _ _ _ _ _ _ _ _ _ _}.
 End FundTm.
 
 Export FundTm(FundTm,Build_FundTm).
 
 Module FundTmEq.
-  Record FundTmEq `{ta : tag} `{WfContext ta} `{WfType ta} `{Typing ta}
-    `{ConvType ta} `{ConvTerm ta} `{ConvNeu ta} `{RedType ta} `{RedTerm ta}
+  Record FundTmEq `{GenericTypingProperties}
     {Γ : context} {A t u : term}
   : Type := {
     VΓ : [||-v Γ ];
@@ -66,7 +60,7 @@ Module FundTmEq.
     Vu : [ Γ ||-v< one > u : A | VΓ | VA ];
     Vtu : [ Γ ||-v< one > t ≅ u : A | VΓ | VA ];
   }.
-  Arguments FundTmEq {_ _ _ _ _ _ _ _ _}.  
+  Arguments FundTmEq {_ _ _ _ _ _ _ _ _ _ _ _}.
 End FundTmEq.
 
 Export FundTmEq(FundTmEq,Build_FundTmEq).
@@ -79,14 +73,196 @@ Section Fundamental.
     since we will reason by induction on them *)
   Import DeclarativeTypingData.
 
+  Lemma FundConNil : FundCon ε.
+  Proof.
+  unshelve econstructor.
+  + unshelve econstructor.
+    - intros; exact unit.
+    - intros; exact unit.
+  + constructor.
+  Qed.
+
+  Lemma FundConCons : forall (Γ : context) (na : aname) (A : term),
+  [ |-[ de ] Γ] -> FundCon Γ -> [Γ |-[ de ] A] -> FundTy Γ A -> FundCon (Γ,, vass na A).
+  Proof.
+  Admitted.
+
+  Lemma FundTyU : forall (Γ : context),
+    [ |-[ de ] Γ] -> FundCon Γ -> FundTy Γ U.
+  Proof.
+  Admitted.
+
+  Lemma FundTyPi : forall (Γ : context) (na : aname) (A B : term),
+    [Γ |-[ de ] A] -> FundTy Γ A ->
+    [Γ,, vass na A |-[ de ] B] -> FundTy (Γ,, vass na A) B ->
+    FundTy Γ (tProd na A B).
+  Proof.
+  Admitted.
+
+  Lemma FundTyUniv : forall (Γ : context) (A : term),
+    [Γ |-[ de ] A : U] -> FundTm Γ U A -> FundTy Γ A.
+  Proof.
+  Admitted.
+
+  Lemma FundTmVar : forall (Γ : context) (n : nat) (decl : context_decl),
+    [ |-[ de ] Γ] -> FundCon Γ ->
+    in_ctx Γ n decl -> FundTm Γ (decl_type decl) (tRel n).
+  Proof.
+  Admitted.
+
+  Lemma FundTmProd : forall (Γ : context) (na : aname) (A B : term),
+    [Γ |-[ de ] A : U] -> FundTm Γ U A ->
+    [Γ,, vass na A |-[ de ] B : U] ->
+    FundTm (Γ,, vass na A) U B -> FundTm Γ U (tProd na A B).
+  Proof.
+  Admitted.
+
+  Lemma FundTmLambda : forall (Γ : context) (na : aname) (A B t : term),
+    [Γ |-[ de ] A] ->
+    FundTy Γ A ->
+    [Γ,, vass na A |-[ de ] t : B] ->
+    FundTm (Γ,, vass na A) B t -> FundTm Γ (tProd na A B) (tLambda na A t).
+  Proof.
+  Admitted.
+
+  Lemma FundTmApp : forall (Γ : context) (na : aname) (f a A B : term),
+    [Γ |-[ de ] f : tProd na A B] ->
+    FundTm Γ (tProd na A B) f ->
+    [Γ |-[ de ] a : A] -> FundTm Γ A a -> FundTm Γ B[a..] (tApp f a).
+  Proof.
+  Admitted.
+
+  Lemma FundTmConv : forall (Γ : context) (t A B : term),
+    [Γ |-[ de ] t : A] -> FundTm Γ A t ->
+    [Γ |-[ de ] A ≅ B] -> FundTyEq Γ A B -> FundTm Γ B t.
+  Proof.
+  Admitted.
+
+  Lemma FundTyEqPiCong : forall (Γ : context) (na nb : aname) (A B C D : term),
+    [Γ |-[ de ] A] ->
+    FundTy Γ A ->
+    [Γ |-[ de ] A ≅ B] ->
+    FundTyEq Γ A B ->
+    [Γ,, vass na A |-[ de ] C ≅ D] ->
+    FundTyEq (Γ,, vass na A) C D -> FundTyEq Γ (tProd na A C) (tProd nb B D).
+  Proof.
+  Admitted.
+
+  Lemma FundTyEqRefl : forall (Γ : context) (A : term),
+    [Γ |-[ de ] A] -> FundTy Γ A -> FundTyEq Γ A A.
+  Proof.
+  Admitted.
+
+  Lemma FundTyEqSym : forall (Γ : context) (A B : term),
+    [Γ |-[ de ] A ≅ B] -> FundTyEq Γ A B -> FundTyEq Γ B A.
+  Proof.
+  Admitted.
+
+  Lemma FundTyEqTrans : forall (Γ : context) (A B C : term),
+    [Γ |-[ de ] A ≅ B] -> FundTyEq Γ A B ->
+    [Γ |-[ de ] B ≅ C] -> FundTyEq Γ B C ->
+    FundTyEq Γ A C.
+  Proof.
+  Admitted.
+
+  Lemma FundTyEqUniv : forall (Γ : context) (A B : term),
+    [Γ |-[ de ] A ≅ B : U] -> FundTmEq Γ U A B -> FundTyEq Γ A B.
+  Proof.
+  Admitted.
+
+  Lemma FundTmEqBRed : forall (Γ : context) (na : aname) (a t A B : term),
+    [Γ |-[ de ] A] ->
+    FundTy Γ A ->
+    [Γ,, vass na A |-[ de ] t : B] ->
+    FundTm (Γ,, vass na A) B t ->
+    [Γ |-[ de ] a : A] ->
+    FundTm Γ A a -> FundTmEq Γ B[a..] (tApp (tLambda na A t) a) t[a..].
+  Proof.
+  Admitted.
+
+  Lemma FundTmEqPiCong : forall (Γ : context) (na nb : aname) (A B C D : term),
+    [Γ |-[ de ] A] -> FundTy Γ A ->
+    [Γ |-[ de ] A ≅ B : U] -> FundTmEq Γ U A B ->
+    [Γ,, vass na A |-[ de ] C ≅ D : U] -> FundTmEq (Γ,, vass na A) U C D ->
+    FundTmEq Γ U (tProd na A C) (tProd nb B D).
+  Proof.
+  Admitted.
+
+  Lemma FundTmEqAppCong : forall (Γ : context) (na : aname) (a b f g A B : term),
+    [Γ |-[ de ] f ≅ g : tProd na A B] -> FundTmEq Γ (tProd na A B) f g ->
+    [Γ |-[ de ] a ≅ b : A] -> FundTmEq Γ A a b ->
+    FundTmEq Γ B[a..] (tApp f a) (tApp g b).
+  Proof.
+  Admitted.
+
+  Lemma FundTmEqFunExt : forall (Γ : context) (na nb : aname) (f g A B : term),
+    [Γ |-[ de ] A] -> FundTy Γ A ->
+    [Γ |-[ de ] f : tProd na A B] -> FundTm Γ (tProd na A B) f ->
+    [Γ |-[ de ] g : tProd nb A B] -> FundTm Γ (tProd nb A B) g ->
+    [Γ,, vass na A |-[ de ] tApp (⟨↑⟩ f) (tRel 0) ≅ tApp (⟨↑⟩ g) (tRel 0) : B] -> FundTmEq (Γ,, vass na A) B (tApp (⟨↑⟩ f) (tRel 0)) (tApp (⟨↑⟩ g) (tRel 0)) ->
+    FundTmEq Γ (tProd na A B) f g.
+  Proof.
+  Admitted.
+
+  Lemma FundTmEqRefl : forall (Γ : context) (t A : term),
+    [Γ |-[ de ] t : A] -> FundTm Γ A t ->
+    FundTmEq Γ A t t.
+  Proof.
+  Admitted.
+
+  Lemma FundTmEqSym : forall (Γ : context) (t t' A : term),
+    [Γ |-[ de ] t ≅ t' : A] -> FundTmEq Γ A t t' ->
+    FundTmEq Γ A t' t.
+  Proof.
+  Admitted.
+
+  Lemma FundTmEqTrans : forall (Γ : context) (t t' t'' A : term),
+    [Γ |-[ de ] t ≅ t' : A] -> FundTmEq Γ A t t' ->
+    [Γ |-[ de ] t' ≅ t'' : A] -> FundTmEq Γ A t' t'' ->
+    FundTmEq Γ A t t''.
+  Proof.
+  Admitted.
+
+  Lemma FundTmEqConv : forall (Γ : context) (t t' A B : term),
+    [Γ |-[ de ] t ≅ t' : A] -> FundTmEq Γ A t t' ->
+    [Γ |-[ de ] A ≅ B] -> FundTyEq Γ A B ->
+    FundTmEq Γ B t t'.
+  Proof.
+  Admitted.
+
+  (* FIXME *)
+  Notation "x × y" := (Datatypes.prod x y) (at level 80, right associativity).
+
   Lemma Fundamental : (forall Γ : context, [ |-[ de ] Γ ] -> FundCon (ta := ta) Γ)
     × (forall (Γ : context) (A : term), [Γ |-[ de ] A] -> FundTy (ta := ta) Γ A)
     × (forall (Γ : context) (A t : term), [Γ |-[ de ] t : A] -> FundTm (ta := ta) Γ A t)
     × (forall (Γ : context) (A B : term), [Γ |-[ de ] A ≅ B] -> FundTyEq (ta := ta) Γ A B)
     × (forall (Γ : context) (A t u : term), [Γ |-[ de ] t ≅ u : A] -> FundTmEq (ta := ta) Γ A t u).
   Proof.
-    apply WfDeclInduction.
-    (*...*)
+  apply WfDeclInduction.
+  + apply FundConNil.
+  + apply FundConCons.
+  + apply FundTyU.
+  + apply FundTyPi.
+  + apply FundTyUniv.
+  + apply FundTmVar.
+  + apply FundTmProd.
+  + apply FundTmLambda.
+  + apply FundTmApp.
+  + apply FundTmConv.
+  + apply FundTyEqPiCong.
+  + apply FundTyEqRefl.
+  + apply FundTyEqSym.
+  + apply FundTyEqTrans.
+  + apply FundTyEqUniv.
+  + apply FundTmEqBRed.
+  + apply FundTmEqPiCong.
+  + apply FundTmEqAppCong.
+  + apply FundTmEqFunExt.
+  + apply FundTmEqRefl.
+  + apply FundTmEqSym.
+  + apply FundTmEqTrans.
+  + apply FundTmEqConv.
   Abort.
-  
+
 End Fundamental.
